\documentclass[11pt]{article}
\usepackage{verbatim}
\usepackage{amsmath}
\begin{document}

Robot game winning probability


\begin{align*}
    % Robot game winning probability
    P(W_{H})&= (1-P(s_1))(1-P(s_2))P(W_H | B_1) + (1-P(s_1))P(s_2)P(W_H | B_2)\\
    &+ P(s_1)(1-P(s_2))P(W_H | B_3) + P(s_1)P(s_2)P(W_H | B_4)\\
    \\
    &= P(B_{1}) * P(W_{H} | B_{1}) + P(B_{2}) * P(W_{H} | B_{2}) \\
    &+ P(B_{3}) * P(W_{H} | B_{3}) + P(B_{4}) * P(W_{H} | B_{4}).
\end{align*}

Since we redo the game when both robots fail, 
\begin{align*}
    P(W_H | B_1) &= P(W_{H})\\
    P(W_H | B_1) &= P(B_{1}) * P(W_{H} | B_{1}) + P(B_{2}) * P(W_{H} | B_{2}) + P(B_{3}) * P(W_{H} | B_{3}) + P(B_{4}) * P(W_{H} | B_{4}).
\end{align*}

.

.


Let
\begin{align*}
    r &= (1-P(s_1))(1-P(s_2))\\
    &= P(B_1)
\end{align*}
\begin{align*}
    u_1 &= P(s_1)P(1-s_2) + P(s_1)P(s_2)P(B_4)\\
    &= P(B_2)P(W_H | B_2) + P(B_3)P(W_H | B_3) + P(B_4)P(W_H | B_4)
\end{align*}



\begin{align*}
    P(W_H | B_1) &= P(B_{1}) * P(W_{H} | B_{1}) + P(B_{2}) * P(W_{H} | B_{2}) + P(B_{3}) * P(W_{H} | B_{3}) + P(B_{4}) * P(W_{H} | B_{4})\\
    &= r(P(W_{H} | B_1)) + u_1\\
    &= u_1 + r(u_1 + u(P(W_{H} | B_1)))\\
    &= u_1 + r(u_1 + r(u_1 + r(u_1 + r\dots)))\\
    &= u_1 + ru_1 + r^2(u_1 + r(u_1 + r\dots))\\
    &= u_1 + ru_1 + r^2 u_1 + r^3 u_1 + r^4 u_1\dots.
\end{align*}
The sum of a geometric series \(y = u_1 (r)^x \) is

\(s_{\infty} = \frac{u_1}{1-r}\),

which I got from the IB Math formula booklet. Since \(r < 1 \), we know that this
series converges and we can use this formula to find a definite answer to this infinite series.
Plugging in actual values in place of stand in variables:
\begin{align*}
    s_{\infty} &= \frac{u_1}{1-r}\\
    &= \frac{P(s_1)P(1-s_2) + P(s_1)P(s_2)P(B_4)}{P(B_1)}\\
    &= \frac{P(s_1)P(1-s_2) + P(s_1)P(s_2)P(B_4)}{1-(1 - P(s_2) - P(s_1) + P(s_1) P(s_2))}\\
    &= \frac{P(s_1)P(1-s_2) + P(s_1)P(s_2)P(B_4)}{P(s_1) + P(s_2) - P(s_1) P(s_2)}
\end{align*}


\begin{equation*}
    % Redo method
    P(W_{H} | B_1) = \frac{(1-s_{A})(s_{B})(B_{2}) + (s_{A})(1-s_{B})(B_{3})+(s_{A})(s_{B})(B_{4})}{s_{A} + s_{B} - (s_{A})(s_{B})}
\end{equation*}

.

.

.

\( P(B_{1}) * P(W_{H} | B_{1})
\)

\end{document}